\begin{footnotesize}
\begin{definition} 
We define the completment of a given set of effects $S$ (under an
execution state $E$) as the super set of $S$, containing ALL the
mid-level effects required to determine ALL the dependencies of the
effects in $S$, i.e.
\begin{fmathpar}
\begin{array}{lll}
S' \in  \left \lceil S \right \rceil \iff  R^{-1}_{S'}(S) = R^{-1}_{E.A}(S)
\end{array}
\end{fmathpar}
\end{definition}

Now, using the above theorem and lemma, we present the proof of the
theorem 3, which starts by listing the following hypotheses and the goal:
\begin{fmathpar}
\begin{array}{ll}
H_0: & \auxred{S} {(\E,op_{<s,i>})} {} {(\E',\eff)}    \\
H_1: & S \cup \{\eta\} \; is \;  \psi\mathtt{-consistent}\\
G_0: & \exists E''.\exists \eta'. \exists V.
((\E,op_{<s,i>})\;\xrightarrow{V}\;(\E'',\eff'))
\end{array}
\end{fmathpar}
Now, by destructing $R$ we get two non-trivial cases:
\begin{itemize}
\item {\bf Case1}($R=\trunc R ;\visZ$):\\
In this case, we generate the premises of the \rulelabel{ub exec} to
achieve the goal. We define the following: 
\begin{fmathpar}
\begin{array}{ll}
H_3: & S' = \left
\lfloor S \right \rfloor_{\mathtt{max}} \\\vspace{1mm}
H_4: & \eta' = F_{op}(S')
\end{array}
\end{fmathpar}




\begin{fmathpar}
\begin{array}{ll}
H_2: & V = S\\
G_1: & \exists E''.\exists \eta'.
((\E,op_{<s,i>})\;\xrightarrow{S}\;(\E'',\eff'))
\end{array}
\end{fmathpar}








\item {\bf Case2}($R=\trunc R;\soZ$):\\
\end{itemize}










\end{footnotesize}
